Integrate CSR with RIoT (#32)

src/riot/RIoT.Core.fst
@@ -30,53 +30,76 @@ module Ed25519 = Hacl.Ed25519
 #restart-solver
 #push-options "--z3rlimit 1024 --fuel 0 --ifuel 0"
 let riot
-(* inputs *)
+(* Common Inputs *)
   (cdi : B.lbuffer byte_sec 32)
   (fwid: B.lbuffer byte_sec 32)
-  (ku: key_usage_payload_t)
-  (version: datatype_of_asn1_type INTEGER)
-  (aliasKeyTBS_template_len: size_t)
-  (aliasKeyTBS_template: B.lbuffer byte_pub (v aliasKeyTBS_template_len))
   (deviceID_label_len: size_t)
   (deviceID_label: B.lbuffer byte_sec (v deviceID_label_len))
   (aliasKey_label_len: size_t)
   (aliasKey_label: B.lbuffer byte_sec (v aliasKey_label_len))
-(* outputs *)
-  (aliasKeyCRT_len: size_t)
-  (aliasKeyCRT_buf: B.lbuffer byte_pub (v aliasKeyCRT_len))
+(* DeviceID CSR Inputs*)
+  (deviceIDCSR_ku: key_usage_payload_t)
+  (deviceIDCSR_version: datatype_of_asn1_type INTEGER)
+  (deviceIDCRI_template_len: size_t)
+  (deviceIDCRI_template: B.lbuffer byte_pub (v deviceIDCRI_template_len))
+(* AliasKey Crt Inputs*)
+  (aliasKeyCrt_ku: key_usage_payload_t)
+  (riot_version: datatype_of_asn1_type INTEGER)
+  (aliasKeyTBS_template_len: size_t)
+  (aliasKeyTBS_template: B.lbuffer byte_pub (v aliasKeyTBS_template_len))
+(* Common Outputs *)
   (aliasKey_pub: B.lbuffer byte_pub 32)
   (aliasKey_priv: B.lbuffer uint8 32)
+(* DeviceID CSR Outputs *)
+  (deviceIDCSR_len: size_t)
+  (deviceIDCSR_buf: B.lbuffer byte_pub (v deviceIDCSR_len))
+(* AliasKey Crt Outputs *)
+  (aliasKeyCRT_len: size_t)
+  (aliasKeyCRT_buf: B.lbuffer byte_pub (v aliasKeyCRT_len))
 : HST.Stack unit
   (requires fun h ->
     B.(all_live h [buf cdi;
                    buf fwid;
-                   buf aliasKeyTBS_template;
                    buf deviceID_label;
                    buf aliasKey_label;
+                   buf deviceIDCRI_template;
+                   buf aliasKeyTBS_template;
+                   buf deviceIDCSR_buf;
                    buf aliasKeyCRT_buf;
                    buf aliasKey_pub;
                    buf aliasKey_priv]) /\
     B.(all_disjoint [loc_buffer cdi;
                      loc_buffer fwid;
-                     loc_buffer aliasKeyTBS_template;
                      loc_buffer deviceID_label;
                      loc_buffer aliasKey_label;
+                     loc_buffer deviceIDCRI_template;
+                     loc_buffer aliasKeyTBS_template;
+                     loc_buffer deviceIDCSR_buf;
                      loc_buffer aliasKeyCRT_buf;
                      loc_buffer aliasKey_pub;
                      loc_buffer aliasKey_priv]) /\
    (* Pre: labels have enough length for HKDF *)
    valid_hkdf_lbl_len deviceID_label_len /\
    valid_hkdf_lbl_len aliasKey_label_len /\
+   (* Pre: DeviceIDCRI template has a valid length *)
+   valid_deviceIDCRI_ingredients deviceIDCRI_template_len deviceIDCSR_version deviceIDCSR_ku /\
+   (* Pre: DeviceIDCSR will have a valid length *)
+   valid_deviceIDCSR_ingredients (len_of_deviceIDCRI deviceIDCRI_template_len deviceIDCSR_version deviceIDCSR_ku) /\
+   (* Pre: `deviceIDCSR_buf` has exact size to write DeviceIDCSR *)
+   v deviceIDCSR_len == length_of_deviceIDCSR (len_of_deviceIDCRI deviceIDCRI_template_len deviceIDCSR_version deviceIDCSR_ku) /\
    (* Pre: AliasKeyTBS template has a valid length *)
-   valid_aliasKeyTBS_ingredients aliasKeyTBS_template_len ku version /\
+   valid_aliasKeyTBS_ingredients aliasKeyTBS_template_len aliasKeyCrt_ku riot_version /\
    (* Pre: AliasKeyTBS will have a valid length *)
-   valid_aliasKeyCRT_ingredients (len_of_aliasKeyTBS aliasKeyTBS_template_len ku version) /\
+   valid_aliasKeyCRT_ingredients (len_of_aliasKeyTBS aliasKeyTBS_template_len aliasKeyCrt_ku riot_version) /\
    (* Pre: `aliasKeyCRT_buf` has exact size to write AliasKeyCRT *)
-   v aliasKeyCRT_len == length_of_aliasKeyCRT (len_of_aliasKeyTBS aliasKeyTBS_template_len ku version)
+   v aliasKeyCRT_len == length_of_aliasKeyCRT (len_of_aliasKeyTBS aliasKeyTBS_template_len aliasKeyCrt_ku riot_version)
    )
    (ensures fun h0 _ h1 ->
     (* Post: Modifies *)
-     B.(modifies (loc_buffer aliasKeyCRT_buf `loc_union` loc_buffer aliasKey_pub `loc_union` loc_buffer aliasKey_priv) h0 h1) /\
+     B.(modifies (loc_buffer deviceIDCSR_buf `loc_union`
+                  loc_buffer aliasKeyCRT_buf `loc_union`
+                  loc_buffer aliasKey_pub    `loc_union`
+                  loc_buffer aliasKey_priv ) h0 h1) /\
     (* Post: AliasKey *)
     ((B.as_seq h1 aliasKey_pub  <: lbytes_pub 32),
      (B.as_seq h1 aliasKey_priv <: lbytes_sec 32)) == derive_AliasKey_spec
@@ -89,25 +112,39 @@ let riot
                                                  (B.as_seq h0 cdi)
                                                  (deviceID_label_len)
                                                  (B.as_seq h0 deviceID_label) in
+     let deviceIDCRI: deviceIDCRI_t deviceIDCRI_template_len = create_deviceIDCRI_spec
+                                                                         (deviceIDCRI_template_len)
+                                                                         (B.as_seq h0 deviceIDCRI_template)
+                                                                         (deviceIDCSR_version)
+                                                                         (deviceIDCSR_ku)
+                                                                         (deviceID_pub_seq)
+                                                                         in
+     let deviceIDCRI_seq = serialize_deviceIDCRI deviceIDCRI_template_len `serialize` deviceIDCRI in
+     let deviceIDCRI_len = len_of_deviceIDCRI deviceIDCRI_template_len deviceIDCSR_version deviceIDCSR_ku in
+     let (* Prf *) _ = lemma_serialize_deviceIDCRI_size_exact deviceIDCRI_template_len deviceIDCRI in
+     let deviceIDCSR: deviceIDCSR_t deviceIDCRI_len = sign_and_finalize_deviceIDCSR_spec
+                                                                (deviceID_priv_seq)
+                                                                (deviceIDCRI_len)
+                                                                (deviceIDCRI_seq) in
      let aliasKeyTBS: aliasKeyTBS_t aliasKeyTBS_template_len = create_aliasKeyTBS_spec
                                                                          (aliasKeyTBS_template_len)
                                                                          (B.as_seq h0 aliasKeyTBS_template)
-                                                                         (ku)
-                                                                         (version)
+                                                                         (aliasKeyCrt_ku)
+                                                                         (riot_version)
                                                                          (B.as_seq h0 fwid)
                                                                          (deviceID_pub_seq)
                                                                          (B.as_seq h1 aliasKey_pub)
                                                                          in
      let aliasKeyTBS_seq = serialize_aliasKeyTBS aliasKeyTBS_template_len `serialize` aliasKeyTBS in
-     let aliasKeyTBS_len = len_of_aliasKeyTBS aliasKeyTBS_template_len ku version in
-     (* Prf *) lemma_serialize_aliasKeyTBS_size_exact aliasKeyTBS_template_len aliasKeyTBS;
-    (let aliasKeyCRT: aliasKeyCRT_t aliasKeyTBS_len = sign_and_finalize_aliasKeyCRT_spec
+     let aliasKeyTBS_len = len_of_aliasKeyTBS aliasKeyTBS_template_len aliasKeyCrt_ku riot_version in
+     let (* Prf *) _ = lemma_serialize_aliasKeyTBS_size_exact aliasKeyTBS_template_len aliasKeyTBS in
+     let aliasKeyCRT: aliasKeyCRT_t aliasKeyTBS_len = sign_and_finalize_aliasKeyCRT_spec
                                                                 (deviceID_priv_seq)
                                                                 (aliasKeyTBS_len)
                                                                 (aliasKeyTBS_seq) in
-     B.as_seq h1 aliasKeyCRT_buf == serialize_aliasKeyCRT aliasKeyTBS_len `serialize` aliasKeyCRT)))
-=
- HST.push_frame ();
+     B.as_seq h1 deviceIDCSR_buf == serialize_deviceIDCSR deviceIDCRI_len `serialize` deviceIDCSR /\
+     B.as_seq h1 aliasKeyCRT_buf == serialize_aliasKeyCRT aliasKeyTBS_len `serialize` aliasKeyCRT))
+= HST.push_frame ();
 
 (* Derive DeviceID *)
   let deviceID_pub : B.lbuffer byte_pub 32 = B.alloca 0x00uy    32ul in
@@ -130,15 +167,37 @@ let riot
     (* lbl *) aliasKey_label_len
               aliasKey_label;
 
+(* Create DeviceIDCRI *)
+   let deviceIDCRI_len: asn1_TLV_int32_of_type SEQUENCE = len_of_deviceIDCRI deviceIDCRI_template_len deviceIDCSR_version deviceIDCSR_ku in
+   let deviceIDCRI_buf: B.lbuffer byte_pub (v deviceIDCRI_len) = B.alloca 0x00uy deviceIDCRI_len in
+
+   printf "Creating DeviceID Certificate Signing Request Information\n" done;
+   create_deviceIDCRI
+    (* version   *) deviceIDCSR_version
+    (* key usage *) deviceIDCSR_ku
+    (* DeviceID  *) deviceID_pub
+    (* Template  *) deviceIDCRI_template_len
+                    deviceIDCRI_template
+    (*DeviceIDCRI*) deviceIDCRI_len
+                    deviceIDCRI_buf;
+
+(* Sign AliasKeyTBS and Finalize AliasKeyCRT *)
+  printf "Signing and finalizing DeviceID Certificate Signing Request\n" done;
+  sign_and_finalize_deviceIDCSR
+    (*Signing Key*) deviceID_priv
+    (*DeviceIDCRI*) deviceIDCRI_len
+                    deviceIDCRI_buf
+    (*DeviceIDCSR*) deviceIDCSR_len
+                    deviceIDCSR_buf;
 (* Create AliasKeyTBS *)
-  let aliasKeyTBS_len: asn1_TLV_int32_of_type SEQUENCE = len_of_aliasKeyTBS aliasKeyTBS_template_len ku version in
+  let aliasKeyTBS_len: asn1_TLV_int32_of_type SEQUENCE = len_of_aliasKeyTBS aliasKeyTBS_template_len aliasKeyCrt_ku riot_version in
   let aliasKeyTBS_buf: B.lbuffer byte_pub (v aliasKeyTBS_len) = B.alloca 0x00uy aliasKeyTBS_len in
 
   printf "Creating AliasKey Certificate TBS\n" done;
   create_aliasKeyTBS
     (* FWID      *) fwid
-    (* key usage *) ku
-    (* Version   *) version
+    (* key usage *) aliasKeyCrt_ku
+    (* version   *) riot_version
     (* DeviceID  *) deviceID_pub
     (* AliasKey  *) aliasKey_pub
     (* Template  *) aliasKeyTBS_template_len
