src/riot/RIoT.X509.fst
@@ -6,3 +6,5 @@ include RIoT.X509.CompositeDeviceID
 include RIoT.X509.Extension
 include RIoT.X509.AliasKeyTBS
 include RIoT.X509.AliasKeyCRT
+include RIoT.X509.DeviceIDCRI
+include RIoT.X509.DeviceIDCSR
